more

theories/persistent/pstore_1.v
@@ -1003,9 +1003,9 @@ Notation node_map V := (gmap node_loc V).
 Notation ref_map V := (gmap ref_loc V).
 Notation node_graph V := (graph node_loc V).
 
-Notation mapping := (ref_map val).
 
 Definition reference_model := (val * generation)%type.
+Notation mapping := (ref_map reference_model).
 
 Definition snapshot_model := (node_loc * mapping * generation)%type.
 Notation snapshots_model := (gset snapshot_model).
@@ -1022,7 +1022,7 @@ Implicit Types j k l n root snaproot : node_loc.
 Implicit Types r : ref_loc.
 Implicit Types v t s : val.
 Implicit Types w : reference_model.
-Implicit Types σ : mapping.
+Implicit Types σ : ref_map val.
 Implicit Types gen snapgen refgen : generation.
 
 Implicit Types g h : graph_store.
@@ -1039,6 +1039,9 @@ Definition vchange_of_edge : ref_diff_edge -> ref_loc * val :=
 
 Definition gchange_of_edge : ref_diff_edge -> ref_loc * generation :=
   fun '(j, (r, (v, gen)), k) => (r, gen).
+
+Definition change_of_edge : ref_diff_edge -> ref_loc * (val * generation) :=
+  fun '(j, (r, x), k) => (r, x).
 
 Class PstoreG Σ `{zoo_G : !ZooG Σ} := {
   #[local] pstore_G_set_G :: MonoSetG Σ snapshot_model ;
@@ -1058,15 +1061,18 @@ Section pstore_G.
   Context `{pstore_G : PstoreG Σ}.
 
   Definition correct_path_diff (M:map_model) (g:graph_store) :=
-    forall n1 (ds : list ref_diff_edge) n2 σ1 σ2,
-      path g n1 ds n2 -> M !! n1 = Some σ1 -> M !! n2 = Some σ2 ->
-      σ1 = (apply_diffl (vchange_of_edge <$> ds) σ2).
+    forall n1 (ds : list ref_diff_edge) n2 x1 x2,
+      path g n1 ds n2 -> M !! n1 = Some x1 -> M !! n2 = Some x2 ->
+      x1 = (apply_diffl (change_of_edge <$> ds) x2).
 
-  Record store_inv (M:map_model) (G:node_generations) (g:graph_store) (root:node_loc) σ ρv :=
+  Definition decomp (M:map_model) root ρv ρg :=
+    exists ρ, M !! root = Some ρ /\ ρv = (fst <$> ρ) /\ ρg = (snd <$> ρ).
+
+  Record store_inv (M:map_model) (G:node_generations) (g:graph_store) (root:node_loc) σ ρv ρg :=
     { si1M : dom M = vertices g ∪ {[root]};
       si1G : dom M = dom G;
       si2 : σ ⊆ ρv;
-      si3 : M !! root = Some ρv ;
+      si3 : decomp M root ρv ρg;
       si4 : correct_path_diff M g
     }.
 
@@ -1074,13 +1080,13 @@ Section pstore_G.
     forall n r w n', edge g n (r,w) n' -> r ∈ X.
 
   Record coherent (M:map_model) ρv ρg g :=
-    { coh1 : forall n σ, M !! n = Some σ -> dom σ = dom ρv;
+    { coh1 : forall n x, M !! n = Some x -> dom x = dom ρv;
       coh2 : references_in g (dom ρv);
       coh3 : dom ρv = dom ρg;
     }.
 
   Definition captured C n :=
-    exists σ gen, (n, σ, gen) ∈ C.
+    exists x gen, (n, x, gen) ∈ C.
 
   (* TODO include in stdpp ?
      https://gitlab.mpi-sws.org/iris/stdpp/-/issues/209 *)
@@ -1160,7 +1166,7 @@ Section pstore_G.
   Qed.
 
   Lemma history_vertices_have_a_generation M C G ρg g root σ ρv h orig :
-    store_inv M G g root σ ρv ->
+    store_inv M G g root σ ρv ρg ->
     history_inv g G ρg root h orig ->
     forall k, k ∈ vertices h ->
     exists kgen, G !! k = Some kgen.
@@ -1196,10 +1202,10 @@ Section pstore_G.
        for a child of the current root. *)
     (gen_succ_rel C G store_gen root).
 
-  Definition snapshot_inv M C G l σ snap_gen :=
-    exists σ',
-      M !! l = Some σ' /\
-      σ ⊆ σ' /\
+  Definition snapshot_inv M C G l x snap_gen :=
+    exists x',
+      M !! l = Some x' /\
+      x ⊆ x' /\
       (* /!\ [snap_gen] is the value store in the [snap_gen] field of
          the snapshot, which corresponds to the current store
          generation *before* the snapshot was captured. It is not in
@@ -1209,13 +1215,13 @@ Section pstore_G.
       gen_succ_rel C G (1 + snap_gen) l.
 
   Definition snapshots_inv M C G :=
-    forall l σ snap_gen, (l, σ, snap_gen) ∈ C ->
-      snapshot_inv M C G l σ snap_gen.
+    forall l x snap_gen, (l, x, snap_gen) ∈ C ->
+      snapshot_inv M C G l x snap_gen.
 
   #[local] Definition pstore_map_auth (γ:gname) (s:gset snapshot_model) :=
     mono_set_auth γ (DfracOwn 1) s.
-  #[local] Definition pstore_map_elem γ l σ gen :=
-    mono_set_elem γ (l, σ, gen).
+  #[local] Definition pstore_map_elem γ l σ gen : iProp Σ:=
+    ∃ x, ⌜σ = fst <$> x⌝ ∗ mono_set_elem γ (l, x, gen).
 
 
   (* FIXME: I don't know how to unfold notations in spatial hypotheses,
@@ -1307,7 +1313,7 @@ Section pstore_G.
       (G:node_generations) (* the generation of each node *)
       ,
     ⌜t=#t0 /\
-     store_inv M G g root σ ρv /\
+     store_inv M G g root σ ρv ρg /\
      topology_inv g M C root /\
      history_inv g G ρg root h orig /\
      coherent M ρv ρg g /\
@@ -1361,6 +1367,12 @@ Section pstore_G.
     lwt_inv {[root := 0]} ∅ [].
   Proof. done. Qed.
 
+  Lemma decomp_init root :
+    decomp {[root := ∅]} root ∅ ∅.
+  Proof.
+    exists ∅. rewrite lookup_insert //.
+  Qed.
+
   Lemma pstore_create_spec :
     {{{ True }}}
       pstore_create ()
@@ -1389,7 +1401,7 @@ Section pstore_G.
       { rewrite dom_singleton_L vertices_empty //. set_solver. }
       { set_solver. }
       { set_solver. }
-      { rewrite lookup_insert //. }
+      { eauto using decomp_init. }
       { intros ????? Hroot.
         rewrite !lookup_singleton_Some.
         inversion Hroot; set_solver. } }
@@ -1430,7 +1442,7 @@ Section pstore_G.
   Lemma use_references_in g n ds n' X :
     references_in g X ->
     path g n ds n' ->
-    (list_to_set (vchange_of_edge <$> ds).*1) ⊆ X.
+    (list_to_set (change_of_edge <$> ds).*1) ⊆ X.
   Proof.
     intros He.
     induction 1; first set_solver.
@@ -1509,7 +1521,7 @@ Section pstore_G.
     iModIntro. iSplitR. { iPureIntro. by eapply not_elem_of_dom. }
     iExists (* r0, root, orig, gen: *) t0, root, orig, gen,
             (* ρv, ρg, g, h: *) (<[r:=v]>ρv), (<[r:=0]>ρg), g, h,
-            (* M, C, G: *) ((fun σ => <[r:=v]>σ)<$> M),C,G.
+            (* M, C, G: *) ((fun x => <[r:=(v,0)]>x)<$> M),C,G.
 
     do 2 rewrite big_sepM_insert //. iFrame "∗".
     iSplitL "Hrest"; [ iPureIntro; split_and!; eauto | eauto ].
@@ -1519,7 +1531,7 @@ Section pstore_G.
       { rewrite dom_fmap_L; set_solver. }
       { rewrite dom_fmap_L; set_solver. }
       { eauto using gmap_included_insert. }
-      { rewrite lookup_fmap X4 //. }
+      { destruct X4 as (x&E1&E2&E3). exists (<[r:=(v,0)]> x). rewrite !lookup_fmap E1 E2 E3 !fmap_insert //. }
       { intros l1 ds l2 σ1 σ2 Hl. rewrite !lookup_fmap. generalize Hl. intros Hreach.
         intros Hl1 Hl2.
         destruct (M !! l1) eqn:Hor1. 2:simpl in *; congruence.
@@ -1551,8 +1563,8 @@ Section pstore_G.
     { (* snapshots_inv *)
       iDestruct "HC" as "[% (%Hsnap&?&?)]".
       iExists γ. iFrame. iPureIntro.
-      intros snaproot ? ? HC. apply Hsnap in HC. destruct HC as (x & Hx & ? & ?).
-      exists (<[r:=v]>x).
+      intros snaproot ? ? HC. apply Hsnap in HC. destruct HC as (x' & Hx & ? & ?).
+      exists (<[r:=(v,0)]>x').
       split_and!; eauto.
       - rewrite lookup_fmap Hx; eauto.
       - apply gmap_included_insert_notin; eauto.
@@ -1562,8 +1574,8 @@ Section pstore_G.
   Qed.
 
 
-  Lemma use_r_in_σ {M G g root} σ ρv r v :
-    store_inv M G g root σ ρv ->
+  Lemma use_r_in_σ {M G g root} σ ρv ρg r v :
+    store_inv M G g root σ ρv ρg ->
     σ !! r = Some v ->
     ρv !! r = Some v.
   Proof.
@@ -1590,7 +1602,7 @@ Section pstore_G.
     wp_rec. iStep 4. iModIntro.
 
     assert (ρv !! r = Some v) as Hρv.
-    { eapply use_r_in_σ with σ; eauto. }
+    { eapply use_r_in_σ with σ _; eauto. }
 
     iDestruct (big_sepM_lookup_acc _ _ r v with "Hρv") as "(H & Hclose)"; eauto.
 
@@ -1672,12 +1684,14 @@ Section pstore_G.
     iModIntro.
 
     set rdiff := (r, (old, refgen)).
+    destruct Hinv as [X1 X2 X3 X4 X5].
+    destruct X4 as (ρ&X41&X42&X43).
 
     iExists (* r0, root, orig, gen: *) t0, newroot, orig, gen,
             (* ρv, ρg: *) (<[r:=v]>ρv), (<[r:=gen]>ρg),
             (* g, h: *)   ({[(root, rdiff, newroot)]} ∪ g),
                           ({[(newroot, rdiff, root)]} ∪ h),
-            (* M, C, G: *) (<[newroot:=<[r:=v]> ρv]>M), C, (<[newroot:=gen]>G).
+            (* M, C, G: *) (<[newroot:=<[r:=(v,gen)]> ρ]>M), C, (<[newroot:=gen]>G).
 
     rewrite big_sepS_union.
     { apply disjoint_singleton_l. intros ?. apply Hnewroot.
@@ -1687,12 +1701,12 @@ Section pstore_G.
     iDestruct "HC" as "[% (%Hsnap&?&?)]".
     { iSplitR; [ iPureIntro; split_and!; first done | eauto ].
     - (* store_inv *)
-      destruct Hinv as [X1 X2 X3 X4 X5].
       constructor.
       { rewrite dom_insert_L vertices_union vertices_singleton //. set_solver. }
       { set_solver. }
       { apply gmap_included_insert. done. }
-      { rewrite lookup_insert //. }
+      { eexists. rewrite lookup_insert X42 X43. split_and !; try done.
+        all:rewrite fmap_insert //. }
       { intros l1 ds l2 σ1 σ2 Hreach.
         destruct_decide (decide (newroot = l1)).
         { subst. rewrite lookup_insert. inversion_clear 1.
@@ -1707,8 +1721,11 @@ Section pstore_G.
           apply path_add_inv_r in Hreach; try done.
           destruct Hreach as [(->&->)|(ds'&->&Hreach)].
           { congruence. }
-          specialize (X5 _ _ _ _ _ Hreach E1 X4).
-          rewrite fmap_app apply_diffl_snoc insert_insert insert_id //. }
+          specialize (X5 _ _ _ _ _ Hreach E1 X41).
+          rewrite fmap_app apply_diffl_snoc insert_insert insert_id //.
+          rewrite lookup_fmap in Hρr.
+          rewrite lookup_fmap in Hrefgen . destruct (ρ !! r) as [(?,?)|] eqn:E; try done.
+          rewrite E. simpl in *. naive_solver. }
         { rewrite lookup_insert_ne //. intros. eapply X5; eauto.
           apply path_cycle_end_inv_aux in Hreach; eauto. } }
     - (* topology_inv *)
@@ -1758,7 +1775,7 @@ Section pstore_G.
           apply mirror_symm.
           assumption.
         }
-      - apply lwt_set; eauto. destruct Hinv. set_solver.
+      - apply lwt_set; eauto. set_solver.
       - rewrite Hhisto.
         unfold undo_graph.
         rewrite list_to_set_cons !list_to_set_app_L. simpl.
@@ -1782,15 +1799,17 @@ Section pstore_G.
         set_solver.
       }
     - (* coherent *)
-      destruct Hcoh as [X1 X2].
-      { constructor.
-      - intros l ?. destruct_decide (decide (l=newroot)).
-        { subst. rewrite lookup_insert. inversion 1. done. }
-        rewrite lookup_insert_ne //. intros HM.
-        apply X1 in HM. rewrite dom_insert_lookup_L //.
-      - intros ?. set_solver.
-      - set_solver.
-      }
+      destruct Hcoh as [Z1 Z2 ?].
+      constructor.
+      { intros l ?. destruct_decide (decide (l=newroot)).
+        { subst. rewrite lookup_insert. inversion 1. subst.
+          rewrite dom_insert_L. set_solver. }
+        { rewrite lookup_insert_ne //. intros HM.
+          apply Z1 in HM. rewrite dom_insert_lookup_L //. } }
+      { intros ????. rewrite dom_insert_L. clear X1 X2 X3.
+        rewrite /edge !elem_of_union.
+        intros [|]; first set_solver. right. eapply Z2. done. }
+      { set_solver. }
     - (* rooted_dag *)
       eauto using rooted_dag_add.
     - (* gen orig *)
@@ -1806,8 +1825,6 @@ Section pstore_G.
           destruct (Hsnap newroot σ' nrgen HnrC) as (σ'', (H', _)).
           eexists; eauto.
         }
-        destruct Hinv.
-        erewrite -> si1M0 in HnrM.
         set_solver.
       }
       { constructor.
@@ -1850,15 +1867,18 @@ Section pstore_G.
       unfold snapshot_inv. destruct HC as (?&HC&?&?).
       assert (r0 ≠ newroot) as Hneqr0nr.
       { intro Hr0r.
-        subst. destruct Hinv as [X1 X2 X3].
+        subst.
         assert (newroot ∉ dom M) as F by set_solver. apply F. by eapply elem_of_dom. }
       rewrite lookup_insert_ne //.
-      exists x.
-      split_and!; eauto; [].
+      exists x0.
+      split_and!; eauto.
       unfold gen_succ_rel.
       rewrite lookup_insert_ne //.
     }
   Qed.
+
+  Definition restrict `{Countable K} {V} (x:gset K) (m:gmap K V) :=
+    map_filter (fun '(k,_) => k ∈ x) _ m.
 
   Lemma pstore_capture_spec t σ :
     {{{
@@ -1875,12 +1895,17 @@ Section pstore_G.
     wp_rec.
     wp_load. wp_store. wp_load. iStep 5.
 
-    iDestruct "HC" as "[% (%Hsnap & Hmeta & HC)]".
-    iMod (mono_set_insert' (root, σ, gen) with "HC") as "(HC&Hsnap)".
+    destruct (si3 _ _ _ _ _ _ _ Hinv) as (ρ&T1&T2&T3).
+    iDestruct "HC" as "[% (%Hsnap & #Hmeta & HC)]".
+    Search restrict.
+    iMod (mono_set_insert' (root, (restrict (dom σ) ρ), gen) with "HC") as "(HC&Hsnap)".
     iModIntro.
-    iSplit. 2:iSteps.
+    iSplit; last first.
+    { unfold pstore_snapshot. iExists _,t0,root,gen. iFrame "Hmeta".
+      iSplitR; first done. iExists _. iFrame.
+      iPureIntro. admit. (* EASY *) }
 
-    set C' : snapshots_model := {[(root, σ, gen)]} ∪ C.
+    set C' : snapshots_model := {[(root, (restrict (dom σ) ρ), gen)]} ∪ C.
 
     assert (gen_succ_rel C' G (1 + gen) root) as HgenC'root. {
       destruct Hglobgen as [Hglobgen1 Hglobgen2].
@@ -1896,10 +1921,34 @@ Section pstore_G.
     iExists (* r0, root, orig, gen: *) t0, root, orig, (1+gen),
             (* ρv, ρg: *) _, _,
             (* g, h: *)   _, _,
-            (* M, C, G: *) _, C', _.
-
-    { iSteps; iPureIntro.
-
+            (* M, C, G: *) M, C', G.
+    iSplitR; last first.
+    { iFrame. iSplitL "Hgen"; first iSteps. iExists _. iFrame "#∗".
+      iPureIntro.
+      (* snapshots_inv M C' G *)
+      intros snaproot ? ? HC. rewrite elem_of_union elem_of_singleton in HC.
+      { destruct HC as [HC|HC].
+      - inversion HC. subst. destruct Hinv.
+        destruct Hglobgen as [Hglobgen1 Hglobgen2].
+        eexists. split_and!; eauto.
+        admit. (* EASY *)
+      - destruct (Hsnap snaproot x snap_gen) as (σ' & HMr' & Hσ' & Hsnapgen); eauto.
+        exists σ'; split_and!; eauto.
+        unfold gen_succ_rel.
+        unfold gen_succ_rel in Hsnapgen.
+        destruct (G !! snaproot) as [ gsnaproot | ]; eauto.
+        assert (captured C snaproot <-> captured C' snaproot) as CAPequiv. {
+          destruct_decide (decide (root = snaproot)).
+          - subst root.
+            unfold captured; set_solver.
+          - unfold C'.
+            unfold captured; set_solver.
+        }
+        { destruct_decide (decide (captured C snaproot)) as CAP; rewrite CAPequiv in CAP.
+        - rewrite decide_True //.
+        - rewrite decide_False //.
+        } } }
+    { iPureIntro. split_and !; try done.
     - (* topology_inv g M C' *)
       intros l Hl_dom Hl_cap.
       assert (not (captured C l)) as CAPl
@@ -1907,7 +1956,8 @@ Section pstore_G.
       apply (Htopo l Hl_dom CAPl).
 
     (* global_gen_inv. *)
-    - (* gen_succ_rel between nodes (k, l) *)
+    - split; try done.
+      + (* gen_succ_rel between nodes (k, l) *)
       destruct Hglobgen as (Hglobgen1 & Hglobgen2).
       intros k gk l Hkl Hgk.
       unfold gen_succ_rel.
@@ -1948,29 +1998,6 @@ Section pstore_G.
         - rewrite decide_False; eauto.
         }
       }
-
-    - (* snapshots_inv M C' G *)
-      intros snaproot ? ? HC. rewrite elem_of_union elem_of_singleton in HC.
-      { destruct HC as [HC|HC].
-      - inversion HC. subst. destruct Hinv.
-        destruct Hglobgen as [Hglobgen1 Hglobgen2].
-        exists ρv; split_and!; eauto.
-      - destruct (Hsnap snaproot σ0 snap_gen) as (σ' & HMr' & Hσ' & Hsnapgen); eauto.
-        exists σ'; split_and!; eauto.
-        unfold gen_succ_rel.
-        unfold gen_succ_rel in Hsnapgen.
-        destruct (G !! snaproot) as [ gsnaproot | ]; eauto.
-        assert (captured C snaproot <-> captured C' snaproot) as CAPequiv. {
-          destruct_decide (decide (root = snaproot)).
-          - subst root.
-            unfold captured; set_solver.
-          - unfold C'.
-            unfold captured; set_solver.
-        }
-        { destruct_decide (decide (captured C snaproot)) as CAP; rewrite CAPequiv in CAP.
-        - rewrite decide_True //.
-        - rewrite decide_False //.
-        }
     }
   Admitted.
 
